#198 done: generic abp with instantiation

abp/ABPComponent.thy
@@ -3,25 +3,26 @@
  * This file was generated from ABP.maa and will be overridden when changed. To change
  * permanently, consider changing the model itself.
  *
- * isartransformer 1.0.0
+ * Generated on Sep 29, 2018 5:54:16 PM by isartransformer 1.0.0
  *)
 theory ABPComponent
-  imports ReceiverAutomaton SenderAutomaton MediumAutomaton
+  imports SenderAutomaton MediumAutomaton ReceiverAutomaton spec.SPS
 
 begin
 
-(* Dummy *)
-definition uspecComp :: "('m,'m) ufun uspec \<Rightarrow> ('m,'m) ufun uspec \<Rightarrow> ('m,'m) ufun uspec" (infixl "\<Otimes>" 50) where
-"uspecComp S1 S2 \<equiv> undefined"
 
 (* Dummy *)
-definition spf2Sps :: "('m,'m) SPF \<Rightarrow> 'm SPS" where
-"spf2Sps f = undefined"
+definition uspecComp :: "('m,'m) ufun uspec ⇒ ('m,'m) ufun uspec ⇒ ('m,'m) ufun uspec" (infixl "⨂" 50) where
+"uspecComp S1 S2 ≡ undefined"
+
+(* Dummy *)
+definition uspecSerComp :: "('in,'m) ufun uspec ⇒ ('m,'out) ufun uspec ⇒ ('in,'out) ufun uspec" (infixl "○" 50) where
+"uspecSerComp S1 S2 ≡ undefined"
 
 
-section \<open>Datatype definition\<close>
+section ‹Datatype definition›
 
-datatype ('e::countable) abpMessage = AbpPair_E_Bool "('e\<times>bool)" | AbpBool "bool" | AbpE "'e"
+datatype ('e::countable) abpMessage = DoNotUse_5b2352bc0cd24bc7b6c3f6f480670fcb_ABPE "'e" | DoNotUse_5b2352bc0cd24bc7b6c3f6f480670fcb_ABPBool "bool" | DoNotUse_5b2352bc0cd24bc7b6c3f6f480670fcb_ABPPair_E_Bool "('e×bool)"
 
 instance abpMessage :: (countable) countable
   apply(intro_classes)
@@ -29,106 +30,552 @@ instance abpMessage :: (countable) countable
 
 instantiation abpMessage :: (countable) message
 begin
-  fun ctype_abpMessage :: "channel \<Rightarrow> ('e::countable) abpMessage set" where
+  fun ctype_abpMessage :: "channel ⇒ ('e::countable) abpMessage set" where
   "ctype_abpMessage c = (
-    if c = \<C> ''sender_i'' then range AbpE else
-    if c = \<C> ''sender_ds__mediumSr_ar'' then range AbpPair_E_Bool else
-    if c = \<C> ''mediumSr_as__receiver_dr'' then range AbpPair_E_Bool else
-    if c = \<C> ''receiver_ar__mediumRs_ar'' then range AbpBool else
-    if c = \<C> ''receiver_o'' then range AbpE else
-    if c = \<C> ''mediumRs_as__sender_as'' then range AbpBool else
+    if c = 𝒞 ''DoNotUse_5b2352bc0cd24bc7b6c3f6f480670fcb_receiver_o__o'' then range DoNotUse_5b2352bc0cd24bc7b6c3f6f480670fcb_ABPE else
+    if c = 𝒞 ''DoNotUse_5b2352bc0cd24bc7b6c3f6f480670fcb_i__sender_i'' then range DoNotUse_5b2352bc0cd24bc7b6c3f6f480670fcb_ABPE else
+    if c = 𝒞 ''DoNotUse_5b2352bc0cd24bc7b6c3f6f480670fcb_sender_ds__mediumSr_ar'' then range DoNotUse_5b2352bc0cd24bc7b6c3f6f480670fcb_ABPPair_E_Bool else
+    if c = 𝒞 ''DoNotUse_5b2352bc0cd24bc7b6c3f6f480670fcb_mediumSr_as__receiver_dr'' then range DoNotUse_5b2352bc0cd24bc7b6c3f6f480670fcb_ABPPair_E_Bool else
+    if c = 𝒞 ''DoNotUse_5b2352bc0cd24bc7b6c3f6f480670fcb_receiver_ar__mediumRs_ar'' then range DoNotUse_5b2352bc0cd24bc7b6c3f6f480670fcb_ABPBool else
+    if c = 𝒞 ''DoNotUse_5b2352bc0cd24bc7b6c3f6f480670fcb_mediumRs_as__sender_as'' then range DoNotUse_5b2352bc0cd24bc7b6c3f6f480670fcb_ABPBool else
     undefined)"
   instance
     by(intro_classes)
 end
 
 
-section \<open>Getter and Setter\<close>
+section ‹Helpers to create a bundle from a single raw element›
 
-(* mediumSr.as \<rightarrow> receiver.dr *)
-lift_definition abp_get_stream_mediumSr_as__receiver_dr :: "('e::countable) abpMessage tsyn SB \<rightarrow> ('e\<times>bool) tsyn stream" is
-"undefined"
+lift_definition aBPElem_raw_receiver_o__o :: "'e ⇒ ('e::countable) abpMessage tsyn sbElem" is
+"λx. [𝒞 ''DoNotUse_5b2352bc0cd24bc7b6c3f6f480670fcb_receiver_o__o'' ↦ Msg (DoNotUse_5b2352bc0cd24bc7b6c3f6f480670fcb_ABPE x)]"
+  unfolding sbElemWell_def
+  unfolding usclOkay_stream_def
+  unfolding ctype_tsyn_def
+  by simp
+
+lift_definition aBPElem_raw_i__sender_i :: "'e ⇒ ('e::countable) abpMessage tsyn sbElem" is
+"λx. [𝒞 ''DoNotUse_5b2352bc0cd24bc7b6c3f6f480670fcb_i__sender_i'' ↦ Msg (DoNotUse_5b2352bc0cd24bc7b6c3f6f480670fcb_ABPE x)]"
+  unfolding sbElemWell_def
+  unfolding usclOkay_stream_def
+  unfolding ctype_tsyn_def
+  by simp
+
+lift_definition aBPElem_raw_sender_ds__mediumSr_ar :: "('e×bool) ⇒ ('e::countable) abpMessage tsyn sbElem" is
+"λx. [𝒞 ''DoNotUse_5b2352bc0cd24bc7b6c3f6f480670fcb_sender_ds__mediumSr_ar'' ↦ Msg (DoNotUse_5b2352bc0cd24bc7b6c3f6f480670fcb_ABPPair_E_Bool x)]"
+  unfolding sbElemWell_def
+  unfolding usclOkay_stream_def
+  unfolding ctype_tsyn_def
+  by simp
+
+lift_definition aBPElem_raw_mediumSr_as__receiver_dr :: "('e×bool) ⇒ ('e::countable) abpMessage tsyn sbElem" is
+"λx. [𝒞 ''DoNotUse_5b2352bc0cd24bc7b6c3f6f480670fcb_mediumSr_as__receiver_dr'' ↦ Msg (DoNotUse_5b2352bc0cd24bc7b6c3f6f480670fcb_ABPPair_E_Bool x)]"
+  unfolding sbElemWell_def
+  unfolding usclOkay_stream_def
+  unfolding ctype_tsyn_def
+  by simp
+
+lift_definition aBPElem_raw_receiver_ar__mediumRs_ar :: "bool ⇒ ('e::countable) abpMessage tsyn sbElem" is
+"λx. [𝒞 ''DoNotUse_5b2352bc0cd24bc7b6c3f6f480670fcb_receiver_ar__mediumRs_ar'' ↦ Msg (DoNotUse_5b2352bc0cd24bc7b6c3f6f480670fcb_ABPBool x)]"
+  unfolding sbElemWell_def
+  unfolding usclOkay_stream_def
+  unfolding ctype_tsyn_def
+  by simp
+
+lift_definition aBPElem_raw_mediumRs_as__sender_as :: "bool ⇒ ('e::countable) abpMessage tsyn sbElem" is
+"λx. [𝒞 ''DoNotUse_5b2352bc0cd24bc7b6c3f6f480670fcb_mediumRs_as__sender_as'' ↦ Msg (DoNotUse_5b2352bc0cd24bc7b6c3f6f480670fcb_ABPBool x)]"
+  unfolding sbElemWell_def
+  unfolding usclOkay_stream_def
+  unfolding ctype_tsyn_def
+  by simp
+
+
+section ‹Helpers to create a bundle from a single tsyn element›
+
+fun aBPElem_receiver_o__o :: "'e tsyn ⇒ ('e::countable) abpMessage tsyn sbElem" where
+"aBPElem_receiver_o__o (Msg receiver_port_o__port_o) = aBPElem_raw_receiver_o__o receiver_port_o__port_o" |
+"aBPElem_receiver_o__o null = sbeNull {𝒞 ''DoNotUse_5b2352bc0cd24bc7b6c3f6f480670fcb_receiver_o__o''}"
+
+declare aBPElem_receiver_o__o.simps[simp del]
+
+definition aBP_receiver_o__o :: "'e tsyn ⇒ ('e::countable) abpMessage tsyn SB" where
+"aBP_receiver_o__o receiver_port_o__port_o = sbe2SB (aBPElem_receiver_o__o receiver_port_o__port_o)"
+
+fun aBPElem_i__sender_i :: "'e tsyn ⇒ ('e::countable) abpMessage tsyn sbElem" where
+"aBPElem_i__sender_i (Msg port_i__sender_port_i) = aBPElem_raw_i__sender_i port_i__sender_port_i" |
+"aBPElem_i__sender_i null = sbeNull {𝒞 ''DoNotUse_5b2352bc0cd24bc7b6c3f6f480670fcb_i__sender_i''}"
+
+declare aBPElem_i__sender_i.simps[simp del]
+
+definition aBP_i__sender_i :: "'e tsyn ⇒ ('e::countable) abpMessage tsyn SB" where
+"aBP_i__sender_i port_i__sender_port_i = sbe2SB (aBPElem_i__sender_i port_i__sender_port_i)"
+
+fun aBPElem_sender_ds__mediumSr_ar :: "('e×bool) tsyn ⇒ ('e::countable) abpMessage tsyn sbElem" where
+"aBPElem_sender_ds__mediumSr_ar (Msg sender_port_ds__mediumSr_port_ar) = aBPElem_raw_sender_ds__mediumSr_ar sender_port_ds__mediumSr_port_ar" |
+"aBPElem_sender_ds__mediumSr_ar null = sbeNull {𝒞 ''DoNotUse_5b2352bc0cd24bc7b6c3f6f480670fcb_sender_ds__mediumSr_ar''}"
+
+declare aBPElem_sender_ds__mediumSr_ar.simps[simp del]
+
+definition aBP_sender_ds__mediumSr_ar :: "('e×bool) tsyn ⇒ ('e::countable) abpMessage tsyn SB" where
+"aBP_sender_ds__mediumSr_ar sender_port_ds__mediumSr_port_ar = sbe2SB (aBPElem_sender_ds__mediumSr_ar sender_port_ds__mediumSr_port_ar)"
+
+fun aBPElem_mediumSr_as__receiver_dr :: "('e×bool) tsyn ⇒ ('e::countable) abpMessage tsyn sbElem" where
+"aBPElem_mediumSr_as__receiver_dr (Msg mediumSr_port_as__receiver_port_dr) = aBPElem_raw_mediumSr_as__receiver_dr mediumSr_port_as__receiver_port_dr" |
+"aBPElem_mediumSr_as__receiver_dr null = sbeNull {𝒞 ''DoNotUse_5b2352bc0cd24bc7b6c3f6f480670fcb_mediumSr_as__receiver_dr''}"
+
+declare aBPElem_mediumSr_as__receiver_dr.simps[simp del]
+
+definition aBP_mediumSr_as__receiver_dr :: "('e×bool) tsyn ⇒ ('e::countable) abpMessage tsyn SB" where
+"aBP_mediumSr_as__receiver_dr mediumSr_port_as__receiver_port_dr = sbe2SB (aBPElem_mediumSr_as__receiver_dr mediumSr_port_as__receiver_port_dr)"
+
+fun aBPElem_receiver_ar__mediumRs_ar :: "bool tsyn ⇒ ('e::countable) abpMessage tsyn sbElem" where
+"aBPElem_receiver_ar__mediumRs_ar (Msg receiver_port_ar__mediumRs_port_ar) = aBPElem_raw_receiver_ar__mediumRs_ar receiver_port_ar__mediumRs_port_ar" |
+"aBPElem_receiver_ar__mediumRs_ar null = sbeNull {𝒞 ''DoNotUse_5b2352bc0cd24bc7b6c3f6f480670fcb_receiver_ar__mediumRs_ar''}"
+
+declare aBPElem_receiver_ar__mediumRs_ar.simps[simp del]
+
+definition aBP_receiver_ar__mediumRs_ar :: "bool tsyn ⇒ ('e::countable) abpMessage tsyn SB" where
+"aBP_receiver_ar__mediumRs_ar receiver_port_ar__mediumRs_port_ar = sbe2SB (aBPElem_receiver_ar__mediumRs_ar receiver_port_ar__mediumRs_port_ar)"
+
+fun aBPElem_mediumRs_as__sender_as :: "bool tsyn ⇒ ('e::countable) abpMessage tsyn sbElem" where
+"aBPElem_mediumRs_as__sender_as (Msg mediumRs_port_as__sender_port_as) = aBPElem_raw_mediumRs_as__sender_as mediumRs_port_as__sender_port_as" |
+"aBPElem_mediumRs_as__sender_as null = sbeNull {𝒞 ''DoNotUse_5b2352bc0cd24bc7b6c3f6f480670fcb_mediumRs_as__sender_as''}"
+
+declare aBPElem_mediumRs_as__sender_as.simps[simp del]
+
+definition aBP_mediumRs_as__sender_as :: "bool tsyn ⇒ ('e::countable) abpMessage tsyn SB" where
+"aBP_mediumRs_as__sender_as mediumRs_port_as__sender_port_as = sbe2SB (aBPElem_mediumRs_as__sender_as mediumRs_port_as__sender_port_as)"
+
+(* Create one sbElem for all input channels *)
+definition aBPElemIn_i :: "'e tsyn ⇒ ('e::countable) abpMessage tsyn sbElem" where
+"aBPElemIn_i port_i = (aBPElem_i__sender_i port_i)"
+
+(* Create one sbElem for all output channels *)
+definition aBPElemOut_o :: "'e tsyn ⇒ ('e::countable) abpMessage tsyn sbElem" where
+"aBPElemOut_o port_o = (aBPElem_receiver_o__o port_o)"
+
+(* Create one SB for all input channels *)
+definition aBPIn_i :: "'e tsyn ⇒ ('e::countable) abpMessage tsyn SB" where
+"aBPIn_i port_i = (sbe2SB (aBPElemIn_i port_i))"
+
+(* Create one SB for all output channels *)
+definition aBPOut_o :: "'e tsyn ⇒ ('e::countable) abpMessage tsyn SB" where
+"aBPOut_o port_o = (sbe2SB (aBPElemOut_o port_o))"
+
+
+subsection ‹sender›
+
+(* Create one sbElem for all input channels *)
+definition aBPSenderElemIn_as_i :: "bool tsyn ⇒ 'e tsyn ⇒ ('e::countable) abpMessage tsyn sbElem" where
+"aBPSenderElemIn_as_i port_as port_i = (aBPElem_mediumRs_as__sender_as port_as) ± (aBPElem_i__sender_i port_i)"
+
+(* Create one sbElem for all output channels *)
+definition aBPSenderElemOut_ds :: "('e×bool) tsyn ⇒ ('e::countable) abpMessage tsyn sbElem" where
+"aBPSenderElemOut_ds port_ds = (aBPElem_sender_ds__mediumSr_ar port_ds)"
+
+(* Create one SB for all input channels *)
+definition aBPSenderIn_as_i :: "bool tsyn ⇒ 'e tsyn ⇒ ('e::countable) abpMessage tsyn SB" where
+"aBPSenderIn_as_i port_as port_i = (sbe2SB (aBPSenderElemIn_as_i port_as port_i))"
+
+(* Create one SB for all output channels *)
+definition aBPSenderOut_ds :: "('e×bool) tsyn ⇒ ('e::countable) abpMessage tsyn SB" where
+"aBPSenderOut_ds port_ds = (sbe2SB (aBPSenderElemOut_ds port_ds))"
+
+
+subsection ‹mediumSr›
+
+(* Create one sbElem for all input channels *)
+definition aBPMediumSrElemIn_ar :: "('e×bool) tsyn ⇒ ('e::countable) abpMessage tsyn sbElem" where
+"aBPMediumSrElemIn_ar port_ar = (aBPElem_sender_ds__mediumSr_ar port_ar)"
+
+(* Create one sbElem for all output channels *)
+definition aBPMediumSrElemOut_as :: "('e×bool) tsyn ⇒ ('e::countable) abpMessage tsyn sbElem" where
+"aBPMediumSrElemOut_as port_as = (aBPElem_mediumSr_as__receiver_dr port_as)"
+
+(* Create one SB for all input channels *)
+definition aBPMediumSrIn_ar :: "('e×bool) tsyn ⇒ ('e::countable) abpMessage tsyn SB" where
+"aBPMediumSrIn_ar port_ar = (sbe2SB (aBPMediumSrElemIn_ar port_ar))"
+
+(* Create one SB for all output channels *)
+definition aBPMediumSrOut_as :: "('e×bool) tsyn ⇒ ('e::countable) abpMessage tsyn SB" where
+"aBPMediumSrOut_as port_as = (sbe2SB (aBPMediumSrElemOut_as port_as))"
+
+
+subsection ‹receiver›
+
+(* Create one sbElem for all input channels *)
+definition aBPReceiverElemIn_dr :: "('e×bool) tsyn ⇒ ('e::countable) abpMessage tsyn sbElem" where
+"aBPReceiverElemIn_dr port_dr = (aBPElem_mediumSr_as__receiver_dr port_dr)"
+
+(* Create one sbElem for all output channels *)
+definition aBPReceiverElemOut_ar_o :: "bool tsyn ⇒ 'e tsyn ⇒ ('e::countable) abpMessage tsyn sbElem" where
+"aBPReceiverElemOut_ar_o port_ar port_o = (aBPElem_receiver_ar__mediumRs_ar port_ar) ± (aBPElem_receiver_o__o port_o)"
+
+(* Create one SB for all input channels *)
+definition aBPReceiverIn_dr :: "('e×bool) tsyn ⇒ ('e::countable) abpMessage tsyn SB" where
+"aBPReceiverIn_dr port_dr = (sbe2SB (aBPReceiverElemIn_dr port_dr))"
+
+(* Create one SB for all output channels *)
+definition aBPReceiverOut_ar_o :: "bool tsyn ⇒ 'e tsyn ⇒ ('e::countable) abpMessage tsyn SB" where
+"aBPReceiverOut_ar_o port_ar port_o = (sbe2SB (aBPReceiverElemOut_ar_o port_ar port_o))"
+
+
+subsection ‹mediumRs›
+
+(* Create one sbElem for all input channels *)
+definition aBPMediumRsElemIn_ar :: "bool tsyn ⇒ ('e::countable) abpMessage tsyn sbElem" where
+"aBPMediumRsElemIn_ar port_ar = (aBPElem_receiver_ar__mediumRs_ar port_ar)"
+
+(* Create one sbElem for all output channels *)
+definition aBPMediumRsElemOut_as :: "bool tsyn ⇒ ('e::countable) abpMessage tsyn sbElem" where
+"aBPMediumRsElemOut_as port_as = (aBPElem_mediumRs_as__sender_as port_as)"
+
+(* Create one SB for all input channels *)
+definition aBPMediumRsIn_ar :: "bool tsyn ⇒ ('e::countable) abpMessage tsyn SB" where
+"aBPMediumRsIn_ar port_ar = (sbe2SB (aBPMediumRsElemIn_ar port_ar))"
+
+(* Create one SB for all output channels *)
+definition aBPMediumRsOut_as :: "bool tsyn ⇒ ('e::countable) abpMessage tsyn SB" where
+"aBPMediumRsOut_as port_as = (sbe2SB (aBPMediumRsElemOut_as port_as))"
+
+
+section ‹Helpers to create a bundle from a tsyn stream of elements›
+
+lift_definition DoNotUse_5b2352bc0cd24bc7b6c3f6f480670fcb_aBP_stream_receiver_o__o_h :: "'e tsyn stream ⇒ ('e::countable) abpMessage tsyn SB" is
+"λ s. [(𝒞 ''DoNotUse_5b2352bc0cd24bc7b6c3f6f480670fcb_receiver_o__o'') ↦ (tsynMap (DoNotUse_5b2352bc0cd24bc7b6c3f6f480670fcb_ABPE)⋅s)]"
+  unfolding ubWell_def usclOkay_stream_def ctype_tsyn_def
+  apply auto
   sorry
 
-(* i \<rightarrow> sender.i *)
-lift_definition abp_get_stream_i__sender_i :: "('e::countable) abpMessage tsyn SB \<rightarrow> 'e tsyn stream" is
-"undefined"
+lift_definition aBP_stream_receiver_o__o :: "('e) tsyn stream → ('e::countable) abpMessage tsyn SB" is
+"DoNotUse_5b2352bc0cd24bc7b6c3f6f480670fcb_aBP_stream_receiver_o__o_h"
   sorry
 
-(* mediumRs.as \<rightarrow> sender.as *)
-lift_definition abp_get_stream_mediumRs_as__sender_as :: "('e::countable) abpMessage tsyn SB \<rightarrow> bool tsyn stream" is
-"undefined"
+lift_definition DoNotUse_5b2352bc0cd24bc7b6c3f6f480670fcb_aBP_stream_i__sender_i_h :: "'e tsyn stream ⇒ ('e::countable) abpMessage tsyn SB" is
+"λ s. [(𝒞 ''DoNotUse_5b2352bc0cd24bc7b6c3f6f480670fcb_i__sender_i'') ↦ (tsynMap (DoNotUse_5b2352bc0cd24bc7b6c3f6f480670fcb_ABPE)⋅s)]"
+  unfolding ubWell_def usclOkay_stream_def ctype_tsyn_def
+  apply auto
   sorry
 
-(* sender.ds \<rightarrow> mediumSr.ar *)
-lift_definition abp_get_stream_sender_ds__mediumSr_ar :: "('e::countable) abpMessage tsyn SB \<rightarrow> 'e tsyn stream" is
-"undefined"
+lift_definition aBP_stream_i__sender_i :: "('e) tsyn stream → ('e::countable) abpMessage tsyn SB" is
+"DoNotUse_5b2352bc0cd24bc7b6c3f6f480670fcb_aBP_stream_i__sender_i_h"
   sorry
 
-definition abpReceiverOut_stream_ar_o :: "bool tsyn stream \<rightarrow> 'e tsyn stream \<rightarrow> ('e::countable) abpMessage tsyn SB" where
-"abpReceiverOut_stream_ar_o =  undefined"
+lift_definition DoNotUse_5b2352bc0cd24bc7b6c3f6f480670fcb_aBP_stream_sender_ds__mediumSr_ar_h :: "('e×bool) tsyn stream ⇒ ('e::countable) abpMessage tsyn SB" is
+"λ s. [(𝒞 ''DoNotUse_5b2352bc0cd24bc7b6c3f6f480670fcb_sender_ds__mediumSr_ar'') ↦ (tsynMap (DoNotUse_5b2352bc0cd24bc7b6c3f6f480670fcb_ABPPair_E_Bool)⋅s)]"
+  unfolding ubWell_def usclOkay_stream_def ctype_tsyn_def
+  apply auto
+  sorry
 
-definition abpSenderOut_stream_ds :: "('e\<times>bool) tsyn stream \<rightarrow> 'e abpMessage tsyn SB" where
-"abpSenderOut_stream_ds = undefined"
+lift_definition aBP_stream_sender_ds__mediumSr_ar :: "(('e×bool)) tsyn stream → ('e::countable) abpMessage tsyn SB" is
+"DoNotUse_5b2352bc0cd24bc7b6c3f6f480670fcb_aBP_stream_sender_ds__mediumSr_ar_h"
+  sorry
+
+lift_definition DoNotUse_5b2352bc0cd24bc7b6c3f6f480670fcb_aBP_stream_mediumSr_as__receiver_dr_h :: "('e×bool) tsyn stream ⇒ ('e::countable) abpMessage tsyn SB" is
+"λ s. [(𝒞 ''DoNotUse_5b2352bc0cd24bc7b6c3f6f480670fcb_mediumSr_as__receiver_dr'') ↦ (tsynMap (DoNotUse_5b2352bc0cd24bc7b6c3f6f480670fcb_ABPPair_E_Bool)⋅s)]"
+  unfolding ubWell_def usclOkay_stream_def ctype_tsyn_def
+  apply auto
+  sorry
+
+lift_definition aBP_stream_mediumSr_as__receiver_dr :: "(('e×bool)) tsyn stream → ('e::countable) abpMessage tsyn SB" is
+"DoNotUse_5b2352bc0cd24bc7b6c3f6f480670fcb_aBP_stream_mediumSr_as__receiver_dr_h"
+  sorry
+
+lift_definition DoNotUse_5b2352bc0cd24bc7b6c3f6f480670fcb_aBP_stream_receiver_ar__mediumRs_ar_h :: "bool tsyn stream ⇒ ('e::countable) abpMessage tsyn SB" is
+"λ s. [(𝒞 ''DoNotUse_5b2352bc0cd24bc7b6c3f6f480670fcb_receiver_ar__mediumRs_ar'') ↦ (tsynMap (DoNotUse_5b2352bc0cd24bc7b6c3f6f480670fcb_ABPBool)⋅s)]"
+  unfolding ubWell_def usclOkay_stream_def ctype_tsyn_def
+  apply auto
+  sorry
+
+lift_definition aBP_stream_receiver_ar__mediumRs_ar :: "(bool) tsyn stream → ('e::countable) abpMessage tsyn SB" is
+"DoNotUse_5b2352bc0cd24bc7b6c3f6f480670fcb_aBP_stream_receiver_ar__mediumRs_ar_h"
+  sorry
+
+lift_definition DoNotUse_5b2352bc0cd24bc7b6c3f6f480670fcb_aBP_stream_mediumRs_as__sender_as_h :: "bool tsyn stream ⇒ ('e::countable) abpMessage tsyn SB" is
+"λ s. [(𝒞 ''DoNotUse_5b2352bc0cd24bc7b6c3f6f480670fcb_mediumRs_as__sender_as'') ↦ (tsynMap (DoNotUse_5b2352bc0cd24bc7b6c3f6f480670fcb_ABPBool)⋅s)]"
+  unfolding ubWell_def usclOkay_stream_def ctype_tsyn_def
+  apply auto
+  sorry
+
+lift_definition aBP_stream_mediumRs_as__sender_as :: "(bool) tsyn stream → ('e::countable) abpMessage tsyn SB" is
+"DoNotUse_5b2352bc0cd24bc7b6c3f6f480670fcb_aBP_stream_mediumRs_as__sender_as_h"
+  sorry
+
+(* Create one SB for all input channels *)
+definition aBPIn_stream_i :: "'e tsyn stream → ('e::countable) abpMessage tsyn SB" where
+"aBPIn_stream_i = (Λ  port_i. (aBP_stream_i__sender_i⋅port_i))"
+
+(* Create one SB for all output channels *)
+definition aBPOut_stream_o :: "'e tsyn stream → ('e::countable) abpMessage tsyn SB" where
+"aBPOut_stream_o = (Λ  port_o. (aBP_stream_receiver_o__o⋅port_o))"
 
 
-section \<open>Converter\<close>
+subsection ‹sender›
 
-(* Receiver *)
-lift_definition receiverInConvert::"('e::countable) abpMessage tsyn SB \<rightarrow> 'e receiverMessage tsyn SB" is
-"\<lambda>sb. receiverIn_stream_dr\<cdot>(abp_get_stream_mediumSr_as__receiver_dr\<cdot>sb)"
+(* Create one SB for all input channels *)
+definition aBPSenderIn_stream_as_i :: "bool tsyn stream → 'e tsyn stream → ('e::countable) abpMessage tsyn SB" where
+"aBPSenderIn_stream_as_i = (Λ  port_as port_i. (aBP_stream_mediumRs_as__sender_as⋅port_as) ⊎ (aBP_stream_i__sender_i⋅port_i))"
+
+(* Create one SB for all output channels *)
+definition aBPSenderOut_stream_ds :: "('e×bool) tsyn stream → ('e::countable) abpMessage tsyn SB" where
+"aBPSenderOut_stream_ds = (Λ  port_ds. (aBP_stream_sender_ds__mediumSr_ar⋅port_ds))"
+
+
+subsection ‹mediumSr›
+
+(* Create one SB for all input channels *)
+definition aBPMediumSrIn_stream_ar :: "('e×bool) tsyn stream → ('e::countable) abpMessage tsyn SB" where
+"aBPMediumSrIn_stream_ar = (Λ  port_ar. (aBP_stream_sender_ds__mediumSr_ar⋅port_ar))"
+
+(* Create one SB for all output channels *)
+definition aBPMediumSrOut_stream_as :: "('e×bool) tsyn stream → ('e::countable) abpMessage tsyn SB" where
+"aBPMediumSrOut_stream_as = (Λ  port_as. (aBP_stream_mediumSr_as__receiver_dr⋅port_as))"
+
+
+subsection ‹receiver›
+
+(* Create one SB for all input channels *)
+definition aBPReceiverIn_stream_dr :: "('e×bool) tsyn stream → ('e::countable) abpMessage tsyn SB" where
+"aBPReceiverIn_stream_dr = (Λ  port_dr. (aBP_stream_mediumSr_as__receiver_dr⋅port_dr))"
+
+(* Create one SB for all output channels *)
+definition aBPReceiverOut_stream_ar_o :: "bool tsyn stream → 'e tsyn stream → ('e::countable) abpMessage tsyn SB" where
+"aBPReceiverOut_stream_ar_o = (Λ  port_ar port_o. (aBP_stream_receiver_ar__mediumRs_ar⋅port_ar) ⊎ (aBP_stream_receiver_o__o⋅port_o))"
+
+
+subsection ‹mediumRs›
+
+(* Create one SB for all input channels *)
+definition aBPMediumRsIn_stream_ar :: "bool tsyn stream → ('e::countable) abpMessage tsyn SB" where
+"aBPMediumRsIn_stream_ar = (Λ  port_ar. (aBP_stream_receiver_ar__mediumRs_ar⋅port_ar))"
+
+(* Create one SB for all output channels *)
+definition aBPMediumRsOut_stream_as :: "bool tsyn stream → ('e::countable) abpMessage tsyn SB" where
+"aBPMediumRsOut_stream_as = (Λ  port_as. (aBP_stream_mediumRs_as__sender_as⋅port_as))"
+
+
+section ‹Helpers to get tsyn elements and streams from sbElems and SBs›
+
+fun aBPElem_get_receiver_o__o :: "('e::countable) abpMessage tsyn sbElem ⇒ ('e) tsyn" where
+"aBPElem_get_receiver_o__o sbe = undefined"
+
+lift_definition aBP_get_stream_receiver_o__o :: "('e::countable) abpMessage tsyn SB → 'e tsyn stream" is
+"λsb. tsynMap (inv DoNotUse_5b2352bc0cd24bc7b6c3f6f480670fcb_ABPE)⋅(sb . (𝒞 ''DoNotUse_5b2352bc0cd24bc7b6c3f6f480670fcb_receiver_o__o''))"
+  by(simp add: cfun_def)
+
+fun aBPElem_get_i__sender_i :: "('e::countable) abpMessage tsyn sbElem ⇒ ('e) tsyn" where
+"aBPElem_get_i__sender_i sbe = undefined"
+
+lift_definition aBP_get_stream_i__sender_i :: "('e::countable) abpMessage tsyn SB → 'e tsyn stream" is
+"λsb. tsynMap (inv DoNotUse_5b2352bc0cd24bc7b6c3f6f480670fcb_ABPE)⋅(sb . (𝒞 ''DoNotUse_5b2352bc0cd24bc7b6c3f6f480670fcb_i__sender_i''))"
+  by(simp add: cfun_def)
+
+fun aBPElem_get_sender_ds__mediumSr_ar :: "('e::countable) abpMessage tsyn sbElem ⇒ (('e×bool)) tsyn" where
+"aBPElem_get_sender_ds__mediumSr_ar sbe = undefined"
+
+lift_definition aBP_get_stream_sender_ds__mediumSr_ar :: "('e::countable) abpMessage tsyn SB → ('e×bool) tsyn stream" is
+"λsb. tsynMap (inv DoNotUse_5b2352bc0cd24bc7b6c3f6f480670fcb_ABPPair_E_Bool)⋅(sb . (𝒞 ''DoNotUse_5b2352bc0cd24bc7b6c3f6f480670fcb_sender_ds__mediumSr_ar''))"
+  by(simp add: cfun_def)
+
+fun aBPElem_get_mediumSr_as__receiver_dr :: "('e::countable) abpMessage tsyn sbElem ⇒ (('e×bool)) tsyn" where
+"aBPElem_get_mediumSr_as__receiver_dr sbe = undefined"
+
+lift_definition aBP_get_stream_mediumSr_as__receiver_dr :: "('e::countable) abpMessage tsyn SB → ('e×bool) tsyn stream" is
+"λsb. tsynMap (inv DoNotUse_5b2352bc0cd24bc7b6c3f6f480670fcb_ABPPair_E_Bool)⋅(sb . (𝒞 ''DoNotUse_5b2352bc0cd24bc7b6c3f6f480670fcb_mediumSr_as__receiver_dr''))"
+  by(simp add: cfun_def)
+
+fun aBPElem_get_receiver_ar__mediumRs_ar :: "('e::countable) abpMessage tsyn sbElem ⇒ (bool) tsyn" where
+"aBPElem_get_receiver_ar__mediumRs_ar sbe = undefined"
+
+lift_definition aBP_get_stream_receiver_ar__mediumRs_ar :: "('e::countable) abpMessage tsyn SB → bool tsyn stream" is
+"λsb. tsynMap (inv DoNotUse_5b2352bc0cd24bc7b6c3f6f480670fcb_ABPBool)⋅(sb . (𝒞 ''DoNotUse_5b2352bc0cd24bc7b6c3f6f480670fcb_receiver_ar__mediumRs_ar''))"
+  by(simp add: cfun_def)
+
+fun aBPElem_get_mediumRs_as__sender_as :: "('e::countable) abpMessage tsyn sbElem ⇒ (bool) tsyn" where
+"aBPElem_get_mediumRs_as__sender_as sbe = undefined"
+
+lift_definition aBP_get_stream_mediumRs_as__sender_as :: "('e::countable) abpMessage tsyn SB → bool tsyn stream" is
+"λsb. tsynMap (inv DoNotUse_5b2352bc0cd24bc7b6c3f6f480670fcb_ABPBool)⋅(sb . (𝒞 ''DoNotUse_5b2352bc0cd24bc7b6c3f6f480670fcb_mediumRs_as__sender_as''))"
+  by(simp add: cfun_def)
+
+
+section ‹Converter›
+
+
+subsection ‹sender›
+
+lift_definition senderInConvert :: "('e::countable) abpMessage tsyn SB → ('e) senderMessage tsyn SB" is
+"λsb. senderIn_stream_as_i⋅(aBP_get_stream_mediumRs_as__sender_as⋅sb)⋅(aBP_get_stream_i__sender_i⋅sb)"
   by (simp add: cfun_def)
 
-lift_definition receiverOutConvert::"('e::countable) receiverMessage tsyn SB \<rightarrow> 'e abpMessage tsyn SB" is
-"\<lambda>sb. abpReceiverOut_stream_ar_o\<cdot>(receiver_get_stream_ar\<cdot>sb)\<cdot>(receiver_get_stream_o\<cdot>sb)"
+lift_definition senderOutConvert :: "('e) senderMessage tsyn SB → ('e::countable) abpMessage tsyn SB" is
+"λsb. aBPSenderOut_stream_ds⋅(sender_get_stream_ds⋅sb)"
   by (simp add: cfun_def)
 
-(* Sender *)
-lift_definition senderInConvert::"('e::countable) abpMessage tsyn SB \<rightarrow> 'e senderMessage tsyn SB" is
-"\<lambda>sb. senderIn_stream_as_i\<cdot>(abp_get_stream_mediumRs_as__sender_as\<cdot>sb)\<cdot>(abp_get_stream_i__sender_i\<cdot>sb)"
-  by (simp add: cfun_def)
-
-lift_definition senderOutConvert::"('e::countable) senderMessage tsyn SB \<rightarrow> 'e abpMessage tsyn SB" is
-"\<lambda>sb. abpSenderOut_stream_ds\<cdot>(sender_get_stream_ds\<cdot>sb)"
-  by (simp add: cfun_def)
-
-
-section \<open>Alternative Converter mit Serieller Komposition\<close>
-
-lift_definition receiverInConverterSPF::"('e::countable) abpMessage tsyn SB \<Rrightarrow> 'e receiverMessage tsyn SB" is
-"(\<Lambda> sb . ((ubDom\<cdot>sb = undefined) \<leadsto> receiverInConvert\<cdot>sb))"
+lift_definition senderInConverterSPF :: "('e::countable) abpMessage tsyn SB ⇛ ('e) senderMessage tsyn SB" is
+"(Λ sb . ((ubDom⋅sb = undefined) ↝ senderInConvert⋅sb))"
   sorry
 
-lift_definition receiverOutConverterSPF::"('e::countable) receiverMessage tsyn SB \<Rrightarrow> 'e abpMessage tsyn SB" is
-"(\<Lambda> sb . ((ubDom\<cdot>sb = undefined) \<leadsto> receiverOutConvert\<cdot>sb))"
+lift_definition senderOutConverterSPF :: "('e) senderMessage tsyn SB ⇛ ('e::countable) abpMessage tsyn SB" is
+"(Λ sb . ((ubDom⋅sb = undefined) ↝ senderOutConvert⋅sb))"
   sorry
 
 
-section \<open>Instanzen der Sub-Komponenten\<close>
+subsection ‹mediumSr›
+
+lift_definition mediumSrInConvert :: "('e::countable) abpMessage tsyn SB → (('e×bool)) mediumMessage tsyn SB" is
+"λsb. mediumIn_stream_ar⋅(aBP_get_stream_sender_ds__mediumSr_ar⋅sb)"
+  by (simp add: cfun_def)
+
+lift_definition mediumSrOutConvert :: "(('e×bool)) mediumMessage tsyn SB → ('e::countable) abpMessage tsyn SB" is
+"λsb. aBPMediumSrOut_stream_as⋅(medium_get_stream_as⋅sb)"
+  by (simp add: cfun_def)
+
+lift_definition mediumSrInConverterSPF :: "('e::countable) abpMessage tsyn SB ⇛ (('e×bool)) mediumMessage tsyn SB" is
+"(Λ sb . ((ubDom⋅sb = undefined) ↝ mediumSrInConvert⋅sb))"
+  sorry
+
+lift_definition mediumSrOutConverterSPF :: "(('e×bool)) mediumMessage tsyn SB ⇛ ('e::countable) abpMessage tsyn SB" is
+"(Λ sb . ((ubDom⋅sb = undefined) ↝ mediumSrOutConvert⋅sb))"
+  sorry
+
+
+subsection ‹receiver›
+
+lift_definition receiverInConvert :: "('e::countable) abpMessage tsyn SB → ('e) receiverMessage tsyn SB" is
+"λsb. receiverIn_stream_dr⋅(aBP_get_stream_mediumSr_as__receiver_dr⋅sb)"
+  by (simp add: cfun_def)
+
+lift_definition receiverOutConvert :: "('e) receiverMessage tsyn SB → ('e::countable) abpMessage tsyn SB" is
+"λsb. aBPReceiverOut_stream_ar_o⋅(receiver_get_stream_ar⋅sb)⋅(receiver_get_stream_o⋅sb)"
+  by (simp add: cfun_def)
+
+lift_definition receiverInConverterSPF :: "('e::countable) abpMessage tsyn SB ⇛ ('e) receiverMessage tsyn SB" is
+"(Λ sb . ((ubDom⋅sb = undefined) ↝ receiverInConvert⋅sb))"
+  sorry
+
+lift_definition receiverOutConverterSPF :: "('e) receiverMessage tsyn SB ⇛ ('e::countable) abpMessage tsyn SB" is
+"(Λ sb . ((ubDom⋅sb = undefined) ↝ receiverOutConvert⋅sb))"
+  sorry
+
+
+subsection ‹mediumRs›
+
+lift_definition mediumRsInConvert :: "('e::countable) abpMessage tsyn SB → (bool) mediumMessage tsyn SB" is
+"λsb. mediumIn_stream_ar⋅(aBP_get_stream_receiver_ar__mediumRs_ar⋅sb)"
+  by (simp add: cfun_def)
+
+lift_definition mediumRsOutConvert :: "(bool) mediumMessage tsyn SB → ('e::countable) abpMessage tsyn SB" is
+"λsb. aBPMediumRsOut_stream_as⋅(medium_get_stream_as⋅sb)"
+  by (simp add: cfun_def)
+
+lift_definition mediumRsInConverterSPF :: "('e::countable) abpMessage tsyn SB ⇛ (bool) mediumMessage tsyn SB" is
+"(Λ sb . ((ubDom⋅sb = undefined) ↝ mediumRsInConvert⋅sb))"
+  sorry
+
+lift_definition mediumRsOutConverterSPF :: "(bool) mediumMessage tsyn SB ⇛ ('e::countable) abpMessage tsyn SB" is
+"(Λ sb . ((ubDom⋅sb = undefined) ↝ mediumRsOutConvert⋅sb))"
+  sorry
+
+
+section ‹Instances›
 
 definition sender :: "(('e::countable) abpMessage tsyn, ('e::countable) abpMessage tsyn) SPF" where
-"sender = ufApplyIn senderInConvert\<cdot>(ufApplyOut senderOutConvert\<cdot>senderSPF)"
+"sender = (senderInConverterSPF∘senderSPF∘senderOutConverterSPF)"
 
 definition mediumSr :: "('e::countable) abpMessage tsyn SPS" where
-"mediumSr = undefined"
+"mediumSr = ((uspecConst mediumSrInConverterSPF)○mediumSPS○(uspecConst mediumSrOutConverterSPF))"
 
 definition receiver :: "(('e::countable) abpMessage tsyn, ('e::countable) abpMessage tsyn) SPF" where
-"receiver = ufApplyIn receiverInConvert\<cdot>(ufApplyOut receiverOutConvert\<cdot>receiverSPF)"
+"receiver = (receiverInConverterSPF∘receiverSPF∘receiverOutConverterSPF)"
 
 definition mediumRs :: "('e::countable) abpMessage tsyn SPS" where
-"mediumRs = undefined"
+"mediumRs = ((uspecConst mediumRsInConverterSPF)○mediumSPS○(uspecConst mediumRsOutConverterSPF))"
 
 
-section \<open>Alternative Instanzen mit den alternativen Convertern\<close>
+section ‹Final definition›
 
-definition receiver2 :: "(('e::countable) abpMessage tsyn, ('e::countable) abpMessage tsyn) SPF" where
-"receiver2 = (receiverInConverterSPF \<circ> receiverSPF \<circ> receiverOutConverterSPF)"
+definition aBPSPS :: "('e::countable) abpMessage tsyn SPS" where
+"aBPSPS = ((uspecConst sender)⨂mediumSr⨂(uspecConst receiver)⨂mediumRs)"
 
 
-section \<open>Die Komponente selbst\<close>
+section ‹Lemmas for getter›
 
-definition abp :: "('e::countable) abpMessage tsyn SPS" where
-"abp = (spf2Sps(sender) \<Otimes>  mediumSr \<Otimes>  spf2Sps(receiver) \<Otimes>  mediumRs)"
+subsection ‹Identity lemmas for single sbElems›
+
+lemma abpelem_receiver_o__o_id[simp]: "aBPElem_get_receiver_o__o (aBPElem_receiver_o__o x) = x"
+  sorry
+
+lemma abpelem_i__sender_i_id[simp]: "aBPElem_get_i__sender_i (aBPElem_i__sender_i x) = x"
+  sorry
+
+lemma abpelem_sender_ds__mediumsr_ar_id[simp]: "aBPElem_get_sender_ds__mediumSr_ar (aBPElem_sender_ds__mediumSr_ar x) = x"
+  sorry
+
+lemma abpelem_mediumsr_as__receiver_dr_id[simp]: "aBPElem_get_mediumSr_as__receiver_dr (aBPElem_mediumSr_as__receiver_dr x) = x"
+  sorry
+
+lemma abpelem_receiver_ar__mediumrs_ar_id[simp]: "aBPElem_get_receiver_ar__mediumRs_ar (aBPElem_receiver_ar__mediumRs_ar x) = x"
+  sorry
+
+lemma abpelem_mediumrs_as__sender_as_id[simp]: "aBPElem_get_mediumRs_as__sender_as (aBPElem_mediumRs_as__sender_as x) = x"
+  sorry
+
+
+subsection ‹Identity lemmas for single SBs from streams›
+
+lemma abp_stream_receiver_o__o_id[simp]: "aBP_get_stream_receiver_o__o⋅(aBP_stream_receiver_o__o⋅x) = x"
+  sorry
+
+lemma abp_stream_i__sender_i_id[simp]: "aBP_get_stream_i__sender_i⋅(aBP_stream_i__sender_i⋅x) = x"
+  sorry
+
+lemma abp_stream_sender_ds__mediumsr_ar_id[simp]: "aBP_get_stream_sender_ds__mediumSr_ar⋅(aBP_stream_sender_ds__mediumSr_ar⋅x) = x"
+  sorry
+
+lemma abp_stream_mediumsr_as__receiver_dr_id[simp]: "aBP_get_stream_mediumSr_as__receiver_dr⋅(aBP_stream_mediumSr_as__receiver_dr⋅x) = x"
+  sorry
+
+lemma abp_stream_receiver_ar__mediumrs_ar_id[simp]: "aBP_get_stream_receiver_ar__mediumRs_ar⋅(aBP_stream_receiver_ar__mediumRs_ar⋅x) = x"
+  sorry
+
+lemma abp_stream_mediumrs_as__sender_as_id[simp]: "aBP_get_stream_mediumRs_as__sender_as⋅(aBP_stream_mediumRs_as__sender_as⋅x) = x"
+  sorry
+
+
+subsection ‹Identity lemmas for input sbElems›
+
+lemma abpelemin_i_i__sender_i_id[simp]: "aBPElem_get_i__sender_i (aBPElemIn_i port_i__sender_port_i) = port_i__sender_port_i"
+  sorry
+
+
+subsection ‹Identity lemmas for output sbElems›
+
+lemma abpelemout_o_receiver_o__o_id[simp]: "aBPElem_get_receiver_o__o (aBPElemOut_o receiver_port_o__port_o) = receiver_port_o__port_o"
+  sorry
+
+
+subsection ‹Identity lemmas for input SBs›
+
+lemma abpin_i_i__sender_i_id[simp]: "aBP_get_stream_i__sender_i⋅(aBPIn_i port_i__sender_port_i) = ↑port_i__sender_port_i"
+  sorry
+
+
+subsection ‹Identity lemmas for output SBs›
+
+lemma abpout_o_receiver_o__o_id[simp]: "aBP_get_stream_receiver_o__o⋅(aBPOut_o receiver_port_o__port_o) = ↑receiver_port_o__port_o"
+  sorry
+
+
+subsection ‹Identity lemmas for input SBs from streams›
+
+lemma abpin_stream_i_i__sender_i_id[simp]: "aBP_get_stream_i__sender_i⋅(aBPIn_stream_i⋅port_i__sender_port_i) = port_i__sender_port_i"
+  sorry
+
+
+subsection ‹Identity lemmas for output SBs from streams›
+
+lemma abpout_stream_o_receiver_o__o_id[simp]: "aBP_get_stream_receiver_o__o⋅(aBPOut_stream_o⋅receiver_port_o__port_o) = receiver_port_o__port_o"
+  sorry
 
 
 end
