abp/ReceiverAutomaton.thy
@@ -3,24 +3,13 @@
  * This file was generated from Receiver.maa and will be overridden when changed. To change
  * permanently, consider changing the model itself.
  *
- * Generated on Sep 24, 2018 7:09:25 PM by isartransformer 1.0.0
+ * Generated on Sep 29, 2018 5:54:13 PM by isartransformer 1.0.0
  *)
 theory ReceiverAutomaton
   imports bundle.tsynBundle automat.dAutomaton
 
 begin
 
-
-(* TODO SWS: Move this to dAutomaton *)
-lemma da_h_stepI:
-  assumes "sbeDom sbe = daDom da"
-      and "(daNextOutput da s sbe) = out"
-      and "(daNextState da s sbe) = nextState"
-  shows "spfConcIn (sbe2SB sbe)\<cdot>(da_h da s) = spfConcOut out\<cdot>(da_h da nextState)"
-  by (metis (no_types) assms da_h_dom da_h_final_h3 spfConcIn_dom spfConcIn_step spfConcOut_dom spf_eq)
-
-(* TODO SWS: Move this to...? *)
-setup_lifting type_definition_cfun
 
 (* Helper for easier generation *)
 fun prepend :: "'a::type list \<Rightarrow> 'a \<Rightarrow> 'a list" where
@@ -29,7 +18,7 @@ fun prepend :: "'a::type list \<Rightarrow> 'a \<Rightarrow> 'a list" where
 
 section \<open>Datatype definition\<close>
 
-datatype ('e::countable) receiverMessage = DoNotUse_6bb7a2acb4ad47378fc9b0c670528dcd_ReceiverPair_ReceiverE_ReceiverBool "('e\<times>bool)" | DoNotUse_6bb7a2acb4ad47378fc9b0c670528dcd_ReceiverBool "bool" | DoNotUse_6bb7a2acb4ad47378fc9b0c670528dcd_ReceiverE "'e"
+datatype ('e::countable) receiverMessage = DoNotUse_011016eb91ad4c298d1ab3c92ec5ca28_ReceiverPair_E_Bool "('e\<times>bool)" | DoNotUse_011016eb91ad4c298d1ab3c92ec5ca28_ReceiverBool "bool" | DoNotUse_011016eb91ad4c298d1ab3c92ec5ca28_ReceiverE "'e"
 
 instance receiverMessage :: (countable) countable
   apply(intro_classes)
@@ -39,9 +28,9 @@ instantiation receiverMessage :: (countable) message
 begin
   fun ctype_receiverMessage :: "channel \<Rightarrow> ('e::countable) receiverMessage set" where
   "ctype_receiverMessage c = (
-    if c = \<C> ''DoNotUse_6bb7a2acb4ad47378fc9b0c670528dcd_dr'' then range DoNotUse_6bb7a2acb4ad47378fc9b0c670528dcd_ReceiverPair_ReceiverE_ReceiverBool else
-    if c = \<C> ''DoNotUse_6bb7a2acb4ad47378fc9b0c670528dcd_ar'' then range DoNotUse_6bb7a2acb4ad47378fc9b0c670528dcd_ReceiverBool else
-    if c = \<C> ''DoNotUse_6bb7a2acb4ad47378fc9b0c670528dcd_o'' then range DoNotUse_6bb7a2acb4ad47378fc9b0c670528dcd_ReceiverE else
+    if c = \<C> ''DoNotUse_011016eb91ad4c298d1ab3c92ec5ca28_dr'' then range DoNotUse_011016eb91ad4c298d1ab3c92ec5ca28_ReceiverPair_E_Bool else
+    if c = \<C> ''DoNotUse_011016eb91ad4c298d1ab3c92ec5ca28_ar'' then range DoNotUse_011016eb91ad4c298d1ab3c92ec5ca28_ReceiverBool else
+    if c = \<C> ''DoNotUse_011016eb91ad4c298d1ab3c92ec5ca28_o'' then range DoNotUse_011016eb91ad4c298d1ab3c92ec5ca28_ReceiverE else
     undefined)"
   instance
     by(intro_classes)
@@ -51,21 +40,21 @@ end
 section \<open>Helpers to create a bundle from a single raw element\<close>
 
 lift_definition receiverElem_raw_dr :: "('e\<times>bool) \<Rightarrow> ('e::countable) receiverMessage tsyn sbElem" is
-"\<lambda>x. [\<C> ''DoNotUse_6bb7a2acb4ad47378fc9b0c670528dcd_dr'' \<mapsto> Msg (DoNotUse_6bb7a2acb4ad47378fc9b0c670528dcd_ReceiverPair_ReceiverE_ReceiverBool x)]"
+"\<lambda>x. [\<C> ''DoNotUse_011016eb91ad4c298d1ab3c92ec5ca28_dr'' \<mapsto> Msg (DoNotUse_011016eb91ad4c298d1ab3c92ec5ca28_ReceiverPair_E_Bool x)]"
   unfolding sbElemWell_def
   unfolding usclOkay_stream_def
   unfolding ctype_tsyn_def
   by simp
 
 lift_definition receiverElem_raw_ar :: "bool \<Rightarrow> ('e::countable) receiverMessage tsyn sbElem" is
-"\<lambda>x. [\<C> ''DoNotUse_6bb7a2acb4ad47378fc9b0c670528dcd_ar'' \<mapsto> Msg (DoNotUse_6bb7a2acb4ad47378fc9b0c670528dcd_ReceiverBool x)]"
+"\<lambda>x. [\<C> ''DoNotUse_011016eb91ad4c298d1ab3c92ec5ca28_ar'' \<mapsto> Msg (DoNotUse_011016eb91ad4c298d1ab3c92ec5ca28_ReceiverBool x)]"
   unfolding sbElemWell_def
   unfolding usclOkay_stream_def
   unfolding ctype_tsyn_def
   by simp
 
 lift_definition receiverElem_raw_o :: "'e \<Rightarrow> ('e::countable) receiverMessage tsyn sbElem" is
-"\<lambda>x. [\<C> ''DoNotUse_6bb7a2acb4ad47378fc9b0c670528dcd_o'' \<mapsto> Msg (DoNotUse_6bb7a2acb4ad47378fc9b0c670528dcd_ReceiverE x)]"
+"\<lambda>x. [\<C> ''DoNotUse_011016eb91ad4c298d1ab3c92ec5ca28_o'' \<mapsto> Msg (DoNotUse_011016eb91ad4c298d1ab3c92ec5ca28_ReceiverE x)]"
   unfolding sbElemWell_def
   unfolding usclOkay_stream_def
   unfolding ctype_tsyn_def
@@ -76,7 +65,7 @@ section \<open>Helpers to create a bundle from a single tsyn element\<close>
 
 fun receiverElem_dr :: "('e\<times>bool) tsyn \<Rightarrow> ('e::countable) receiverMessage tsyn sbElem" where
 "receiverElem_dr (Msg port_dr) = receiverElem_raw_dr port_dr" |
-"receiverElem_dr null = sbeNull {\<C> ''DoNotUse_6bb7a2acb4ad47378fc9b0c670528dcd_dr''}"
+"receiverElem_dr null = sbeNull {\<C> ''DoNotUse_011016eb91ad4c298d1ab3c92ec5ca28_dr''}"
 
 declare receiverElem_dr.simps[simp del]
 
@@ -85,7 +74,7 @@ definition receiver_dr :: "('e\<times>bool) tsyn \<Rightarrow> ('e::countable) r
 
 fun receiverElem_ar :: "bool tsyn \<Rightarrow> ('e::countable) receiverMessage tsyn sbElem" where
 "receiverElem_ar (Msg port_ar) = receiverElem_raw_ar port_ar" |
-"receiverElem_ar null = sbeNull {\<C> ''DoNotUse_6bb7a2acb4ad47378fc9b0c670528dcd_ar''}"
+"receiverElem_ar null = sbeNull {\<C> ''DoNotUse_011016eb91ad4c298d1ab3c92ec5ca28_ar''}"
 
 declare receiverElem_ar.simps[simp del]
 
@@ -94,7 +83,7 @@ definition receiver_ar :: "bool tsyn \<Rightarrow> ('e::countable) receiverMessa
 
 fun receiverElem_o :: "'e tsyn \<Rightarrow> ('e::countable) receiverMessage tsyn sbElem" where
 "receiverElem_o (Msg port_o) = receiverElem_raw_o port_o" |
-"receiverElem_o null = sbeNull {\<C> ''DoNotUse_6bb7a2acb4ad47378fc9b0c670528dcd_o''}"
+"receiverElem_o null = sbeNull {\<C> ''DoNotUse_011016eb91ad4c298d1ab3c92ec5ca28_o''}"
 
 declare receiverElem_o.simps[simp del]
 
@@ -118,59 +107,36 @@ definition receiverOut_ar_o :: "bool tsyn \<Rightarrow> 'e tsyn \<Rightarrow> ('
 "receiverOut_ar_o port_ar port_o = (sbe2SB (receiverElemOut_ar_o port_ar port_o))"
 
 
-section \<open>Helpers to create a bundle from a tsyn list of elements\<close>
-
-fun receiver_list_dr :: "(('e\<times>bool) tsyn) list \<Rightarrow> ('e::countable) receiverMessage tsyn SB" where
-"receiver_list_dr (x#xs) = ubConcEq (receiver_dr x)\<cdot>(receiver_list_dr xs)" |
-"receiver_list_dr []     = ubLeast {\<C> ''DoNotUse_6bb7a2acb4ad47378fc9b0c670528dcd_dr''}"
-
-fun receiver_list_ar :: "(bool tsyn) list \<Rightarrow> ('e::countable) receiverMessage tsyn SB" where
-"receiver_list_ar (x#xs) = ubConcEq (receiver_ar x)\<cdot>(receiver_list_ar xs)" |
-"receiver_list_ar []     = ubLeast {\<C> ''DoNotUse_6bb7a2acb4ad47378fc9b0c670528dcd_ar''}"
-
-fun receiver_list_o :: "('e tsyn) list \<Rightarrow> ('e::countable) receiverMessage tsyn SB" where
-"receiver_list_o (x#xs) = ubConcEq (receiver_o x)\<cdot>(receiver_list_o xs)" |
-"receiver_list_o []     = ubLeast {\<C> ''DoNotUse_6bb7a2acb4ad47378fc9b0c670528dcd_o''}"
-
-(* Create one SB for all input channels *)
-definition receiverIn_list_dr :: "('e\<times>bool) tsyn list \<Rightarrow> ('e::countable) receiverMessage tsyn SB" where
-"receiverIn_list_dr port_dr = (receiver_list_dr port_dr)"
-
-(* Create one SB for all output channels *)
-definition receiverOut_list_ar_o :: "bool tsyn list \<Rightarrow> 'e tsyn list \<Rightarrow> ('e::countable) receiverMessage tsyn SB" where
-"receiverOut_list_ar_o port_ar port_o = (receiver_list_ar port_ar) \<uplus> (receiver_list_o port_o)"
-
-
 section \<open>Helpers to create a bundle from a tsyn stream of elements\<close>
 
-lift_definition DoNotUse_6bb7a2acb4ad47378fc9b0c670528dcd_receiver_stream_dr_h :: "('e\<times>bool) tsyn stream \<Rightarrow> ('e::countable) receiverMessage tsyn SB" is
-"\<lambda> s. [(\<C> ''DoNotUse_6bb7a2acb4ad47378fc9b0c670528dcd_dr'') \<mapsto> (tsynMap (DoNotUse_6bb7a2acb4ad47378fc9b0c670528dcd_ReceiverPair_ReceiverE_ReceiverBool)\<cdot>s)]"
+lift_definition DoNotUse_011016eb91ad4c298d1ab3c92ec5ca28_receiver_stream_dr_h :: "('e\<times>bool) tsyn stream \<Rightarrow> ('e::countable) receiverMessage tsyn SB" is
+"\<lambda> s. [(\<C> ''DoNotUse_011016eb91ad4c298d1ab3c92ec5ca28_dr'') \<mapsto> (tsynMap (DoNotUse_011016eb91ad4c298d1ab3c92ec5ca28_ReceiverPair_E_Bool)\<cdot>s)]"
   unfolding ubWell_def usclOkay_stream_def ctype_tsyn_def
   apply auto
   sorry
 
 lift_definition receiver_stream_dr :: "(('e\<times>bool)) tsyn stream \<rightarrow> ('e::countable) receiverMessage tsyn SB" is
-"DoNotUse_6bb7a2acb4ad47378fc9b0c670528dcd_receiver_stream_dr_h"
+"DoNotUse_011016eb91ad4c298d1ab3c92ec5ca28_receiver_stream_dr_h"
   sorry
 
-lift_definition DoNotUse_6bb7a2acb4ad47378fc9b0c670528dcd_receiver_stream_ar_h :: "bool tsyn stream \<Rightarrow> ('e::countable) receiverMessage tsyn SB" is
-"\<lambda> s. [(\<C> ''DoNotUse_6bb7a2acb4ad47378fc9b0c670528dcd_ar'') \<mapsto> (tsynMap (DoNotUse_6bb7a2acb4ad47378fc9b0c670528dcd_ReceiverBool)\<cdot>s)]"
+lift_definition DoNotUse_011016eb91ad4c298d1ab3c92ec5ca28_receiver_stream_ar_h :: "bool tsyn stream \<Rightarrow> ('e::countable) receiverMessage tsyn SB" is
+"\<lambda> s. [(\<C> ''DoNotUse_011016eb91ad4c298d1ab3c92ec5ca28_ar'') \<mapsto> (tsynMap (DoNotUse_011016eb91ad4c298d1ab3c92ec5ca28_ReceiverBool)\<cdot>s)]"
   unfolding ubWell_def usclOkay_stream_def ctype_tsyn_def
   apply auto
   sorry
 
 lift_definition receiver_stream_ar :: "(bool) tsyn stream \<rightarrow> ('e::countable) receiverMessage tsyn SB" is
-"DoNotUse_6bb7a2acb4ad47378fc9b0c670528dcd_receiver_stream_ar_h"
+"DoNotUse_011016eb91ad4c298d1ab3c92ec5ca28_receiver_stream_ar_h"
   sorry
 
-lift_definition DoNotUse_6bb7a2acb4ad47378fc9b0c670528dcd_receiver_stream_o_h :: "'e tsyn stream \<Rightarrow> ('e::countable) receiverMessage tsyn SB" is
-"\<lambda> s. [(\<C> ''DoNotUse_6bb7a2acb4ad47378fc9b0c670528dcd_o'') \<mapsto> (tsynMap (DoNotUse_6bb7a2acb4ad47378fc9b0c670528dcd_ReceiverE)\<cdot>s)]"
+lift_definition DoNotUse_011016eb91ad4c298d1ab3c92ec5ca28_receiver_stream_o_h :: "'e tsyn stream \<Rightarrow> ('e::countable) receiverMessage tsyn SB" is
+"\<lambda> s. [(\<C> ''DoNotUse_011016eb91ad4c298d1ab3c92ec5ca28_o'') \<mapsto> (tsynMap (DoNotUse_011016eb91ad4c298d1ab3c92ec5ca28_ReceiverE)\<cdot>s)]"
   unfolding ubWell_def usclOkay_stream_def ctype_tsyn_def
   apply auto
   sorry
 
 lift_definition receiver_stream_o :: "('e) tsyn stream \<rightarrow> ('e::countable) receiverMessage tsyn SB" is
-"DoNotUse_6bb7a2acb4ad47378fc9b0c670528dcd_receiver_stream_o_h"
+"DoNotUse_011016eb91ad4c298d1ab3c92ec5ca28_receiver_stream_o_h"
   sorry
 
 (* Create one SB for all input channels *)
@@ -188,23 +154,22 @@ fun receiverElem_get_dr :: "('e::countable) receiverMessage tsyn sbElem \<Righta
 "receiverElem_get_dr sbe = undefined"
 
 lift_definition receiver_get_stream_dr :: "('e::countable) receiverMessage tsyn SB \<rightarrow> ('e\<times>bool) tsyn stream" is
-"\<lambda>sb. tsynMap (inv DoNotUse_6bb7a2acb4ad47378fc9b0c670528dcd_ReceiverPair_ReceiverE_ReceiverBool)\<cdot>(sb . (\<C> ''DoNotUse_6bb7a2acb4ad47378fc9b0c670528dcd_dr''))"
+"\<lambda>sb. tsynMap (inv DoNotUse_011016eb91ad4c298d1ab3c92ec5ca28_ReceiverPair_E_Bool)\<cdot>(sb . (\<C> ''DoNotUse_011016eb91ad4c298d1ab3c92ec5ca28_dr''))"
   by(simp add: cfun_def)
 
 fun receiverElem_get_ar :: "('e::countable) receiverMessage tsyn sbElem \<Rightarrow> (bool) tsyn" where
 "receiverElem_get_ar sbe = undefined"
 
 lift_definition receiver_get_stream_ar :: "('e::countable) receiverMessage tsyn SB \<rightarrow> bool tsyn stream" is
-"\<lambda>sb. tsynMap (inv DoNotUse_6bb7a2acb4ad47378fc9b0c670528dcd_ReceiverBool)\<cdot>(sb . (\<C> ''DoNotUse_6bb7a2acb4ad47378fc9b0c670528dcd_ar''))"
+"\<lambda>sb. tsynMap (inv DoNotUse_011016eb91ad4c298d1ab3c92ec5ca28_ReceiverBool)\<cdot>(sb . (\<C> ''DoNotUse_011016eb91ad4c298d1ab3c92ec5ca28_ar''))"
   by(simp add: cfun_def)
 
 fun receiverElem_get_o :: "('e::countable) receiverMessage tsyn sbElem \<Rightarrow> ('e) tsyn" where
 "receiverElem_get_o sbe = undefined"
 
 lift_definition receiver_get_stream_o :: "('e::countable) receiverMessage tsyn SB \<rightarrow> 'e tsyn stream" is
-"\<lambda>sb. tsynMap (inv DoNotUse_6bb7a2acb4ad47378fc9b0c670528dcd_ReceiverE)\<cdot>(sb . (\<C> ''DoNotUse_6bb7a2acb4ad47378fc9b0c670528dcd_o''))"
+"\<lambda>sb. tsynMap (inv DoNotUse_011016eb91ad4c298d1ab3c92ec5ca28_ReceiverE)\<cdot>(sb . (\<C> ''DoNotUse_011016eb91ad4c298d1ab3c92ec5ca28_o''))"
   by(simp add: cfun_def)
-
 
 
 section \<open>Automaton definition\<close>
@@ -239,11 +204,11 @@ fun receiverTransitionH :: "(ReceiverState \<times> (('e\<times>bool) tsyn)) \<R
 
 (* Domain *)
 definition receiverDom :: "channel set" where
-"receiverDom = {\<C> ''DoNotUse_6bb7a2acb4ad47378fc9b0c670528dcd_dr''}"
+"receiverDom = {\<C> ''DoNotUse_011016eb91ad4c298d1ab3c92ec5ca28_dr''}"
 
 (* Range *)
 definition receiverRan :: "channel set" where
-"receiverRan = {\<C> ''DoNotUse_6bb7a2acb4ad47378fc9b0c670528dcd_ar'', \<C> ''DoNotUse_6bb7a2acb4ad47378fc9b0c670528dcd_o''}"
+"receiverRan = {\<C> ''DoNotUse_011016eb91ad4c298d1ab3c92ec5ca28_ar'', \<C> ''DoNotUse_011016eb91ad4c298d1ab3c92ec5ca28_o''}"
 
 (* Transition function *)
 definition receiverTransition :: "(ReceiverState \<times> ('e::countable) receiverMessage tsyn sbElem) \<Rightarrow> (ReceiverState \<times> ('e::countable) receiverMessage tsyn SB)" where
@@ -313,25 +278,25 @@ section \<open>Lemmas for getter\<close>
 
 subsection \<open>Identity lemmas for single sbElems\<close>
 
-lemma receiverelem_dr_id[simp]: "receiverElem_get_dr (receiverElem_dr port_dr) = port_dr"
+lemma receiverelem_dr_id[simp]: "receiverElem_get_dr (receiverElem_dr x) = x"
   sorry
 
-lemma receiverelem_ar_id[simp]: "receiverElem_get_ar (receiverElem_ar port_ar) = port_ar"
+lemma receiverelem_ar_id[simp]: "receiverElem_get_ar (receiverElem_ar x) = x"
   sorry
 
-lemma receiverelem_o_id[simp]: "receiverElem_get_o (receiverElem_o port_o) = port_o"
+lemma receiverelem_o_id[simp]: "receiverElem_get_o (receiverElem_o x) = x"
   sorry
 
 
 subsection \<open>Identity lemmas for single SBs from streams\<close>
 
-lemma receiver_stream_dr_id[simp]: "receiver_get_stream_dr\<cdot>(receiver_stream_dr\<cdot>port_dr) = port_dr"
+lemma receiver_stream_dr_id[simp]: "receiver_get_stream_dr\<cdot>(receiver_stream_dr\<cdot>x) = x"
   sorry
 
-lemma receiver_stream_ar_id[simp]: "receiver_get_stream_ar\<cdot>(receiver_stream_ar\<cdot>port_ar) = port_ar"
+lemma receiver_stream_ar_id[simp]: "receiver_get_stream_ar\<cdot>(receiver_stream_ar\<cdot>x) = x"
   sorry
 
-lemma receiver_stream_o_id[simp]: "receiver_get_stream_o\<cdot>(receiver_stream_o\<cdot>port_o) = port_o"
+lemma receiver_stream_o_id[simp]: "receiver_get_stream_o\<cdot>(receiver_stream_o\<cdot>x) = x"
   sorry
 
 
@@ -362,21 +327,6 @@ lemma receiverout_ar_o_ar_id[simp]: "receiver_get_stream_ar\<cdot>(receiverOut_a
   sorry
 
 lemma receiverout_ar_o_o_id[simp]: "receiver_get_stream_o\<cdot>(receiverOut_ar_o port_ar port_o) = \<up>port_o"
-  sorry
-
-
-subsection \<open>Identity lemmas for input SBs from lists\<close>
-
-lemma receiverin_list_dr_dr_id[simp]: "receiver_get_stream_dr\<cdot>(receiverIn_list_dr port_dr) = <port_dr>"
-  sorry
-
-
-subsection \<open>Identity lemmas for output SBs from lists\<close>
-
-lemma receiverout_list_ar_o_ar_id[simp]: "receiver_get_stream_ar\<cdot>(receiverOut_list_ar_o port_ar port_o) = <port_ar>"
-  sorry
-
-lemma receiverout_list_ar_o_o_id[simp]: "receiver_get_stream_o\<cdot>(receiverOut_list_ar_o port_ar port_o) = <port_o>"
   sorry
 
 
